\documentclass[12pt,a4paper]{article}
\usepackage[dvips]{graphicx,color}
\usepackage{indentfirst}
\usepackage{fancybox}
\usepackage{pslatex}
\usepackage{amsmath}
\usepackage{/Users/lcl/latex/chicago}
\usepackage[left=2.5cm,top=2.3cm,right=2.5cm,nohead,footskip=2cm]{geometry}

\newenvironment{figurehere}
  {\def\@captype{figure}}
  {}
\makeatother

\renewcommand{\baselinestretch}{1.5}

\begin{document}

\begin{flalign}
  - fv & = - \frac{1}{\rho} \frac{\partial p}{\partial x} \\
  fu & = - \frac{1}{\rho} \frac{\partial p}{\partial y}
\end{flalign}

\begin{equation*}
  \frac{\partial}{\partial x} (fu) + \frac{\partial}{\partial} (fv) = - \frac{\partial^2 p}{\partial x \partial y} +   \frac{\partial^2 p}{\partial x \partial y}  
\end{equation*}

\begin{equation*}
  f \frac{\partial u}{\partial x} + u \frac{\partial f}{\partial x} + f \frac{\partial v}{\partial y} + v \frac{\partial f}{\partial y} = 0
\end{equation*}

\begin{equation*}
  f \left( \frac{\partial u}{\partial x} + \frac{\partial v}{\partial y} \right) + \beta v = 0
\end{equation*}

\begin{equation*}
  \beta = \frac{\partial f}{\partial y} = \frac{\partial (2 \Omega \sin \theta)}{\partial y} = \frac{2 \Omega \cos \theta}{R} = 2.3 \times 10^{-11} (\text{m.s})^{-1} \times \cos (\text{latitude}) 
\end{equation*}

\begin{equation*}
  f \frac{\partial w}{\partial z} = \beta v
\end{equation*}

\begin{equation*}
  \int_{z_\text{bottom}}^{z_\text{top}} \beta v dz = \int_{z_\text{bottom}}^{z_\text{top}} f \frac{\partial w}{\partial z} dz
\end{equation*}

\begin{flalign*}
  & \beta V = f w_\text{top}, &
\end{flalign*}

\noindent where $V = \int v dz$, depth-integrated meridional velocity

\begin{flalign}
\setcounter{equation}{2}
  - fv & = \frac{1}{\rho} \frac{\partial \tau_x}{\partial z} \\
  fu & = \frac{1}{\rho} \frac{\partial \tau_y}{\partial z}
\end{flalign}

\begin{equation*}
  \frac{\partial}{\partial x} (fu) + \frac{\partial}{\partial} (fv) = \frac{1}{\rho} \left( \frac{\partial^2 \tau_y}{\partial x \partial z} - \frac{\partial^2 \tau_x}{\partial y \partial z}  \right) 
\end{equation*}

\begin{equation*}
  f \left( \frac{\partial u}{\partial x} + \frac{\partial v}{\partial
    y} \right) + \beta v = \frac{1}{\rho} \\left( \frac{\partial
    \tau_y}{\partial x} - \frac{\partial \tau_x}{\partial y} \right)
\end{equation*}

\begin{equation*}
  - f \frac{\partial w}{\partial z} + \beta v = \frac{1}{\rho} \frac{\partial}{\partial z} \nabla \times 
\tau
\end{equation*}

\begin{equation*}
  \int_{z_\text{Ek}}^{z_0} f \frac{\partial w}{\partial z} dz + \int_{z_\text{Ek}}^{z_0} \beta v dz = \frac{1}{\rho} \int_{z_\text{Ek}}^{z_0} \frac{\partial}{\partial z} \left( \nabla \times \tau \right) dz
\end{equation*}

\begin{equation*}
  - f (0 - w_{Ek}) + \beta V_{Ek} = \frac{1}{\rho} \left( \nabla \times \tau \right) dz
\end{equation*}

\begin{equation*}
  f w_{Ek} - \frac{\beta \tau_x}{\rho f} = \frac{1}{\rho} \left( \nabla \times \tau \right), \text{\: where \;} V_{Ek} = - \frac{\tau_x}{\rho f}
\end{equation*}

\begin{equation*}
  f w_{Ek} - \frac{\beta \tau_x}{\rho f} = \frac{1}{\rho} \left( \nabla \times \tau \right)
\end{equation*}

\begin{equation*}
  f w_{Ek} = \frac{1}{\rho} \left( \nabla \times \tau \right)
\end{equation*}

\begin{flalign*}
  \text{\footnotesize Geostrophic interior: \;\;\;} & \beta V = f w_\text{top} \\
  \text{\footnotesize Ekman layer: \;\;\;} & f w_\text{Ek} = \frac{1}{\rho} \left( \nabla \times \tau \right)
\end{flalign*}


\end{document}
